coq_session/dyn_inv.v
@@ -6,16 +6,16 @@ Set Implicit Arguments.
 Unset Strict Implicit.
 Unset Printing Implicit Defensive.
 
-Lemma dyn_lam0_invX Γ Δ A1 A2 B C m s1 s2 t :
-  Γ ; Δ ⊢ Lam0 A1 m s1 : C ->
+Lemma dyn_lam0_invX Θ Γ Δ A1 A2 B C m s1 s2 t :
+  Θ ; Γ ; Δ ⊢ Lam0 A1 m s1 : C ->
   C === Pi0 A2 B s2 ->
   (A2 :: Γ) ⊢ B : Sort t ->
-  (A2 :: Γ) ; _: Δ ⊢ m : B.
+  Θ ; (A2 :: Γ) ; _: Δ ⊢ m : B.
 Proof with eauto.
   move e:(Lam0 A1 m s1)=>n tyL.
-  elim: tyL A1 A2 B m s1 s2 t e=>//{Γ Δ C n}.
-  { move=>Γ Δ A B m s k tym _ A1 A2 B0 m0
-      s1 s2 t[e1 e2 e3]/pi0_inj[eq1[eq2 e4]]tyB0; subst.
+  elim: tyL A1 A2 B m s1 s2 t e=>//{Θ Γ Δ C n}.
+  { move=>Θ Γ Δ A B m s k1 k2 tym _ A1 A2 B0 m0
+           s1 s2 t[e1 e2 e3]/pi0_inj[eq1[eq2 e4]]tyB0; subst.
     have wf:=dyn_type_wf tym. inv wf.
     have wf:=sta_type_wf tyB0. inv wf.
     apply: dyn_ctx_conv0.
@@ -23,52 +23,177 @@ Proof with eauto.
     exact: H4.
     apply: dyn_conv...
     apply: sta_ctx_conv... }
-  { move=>Γ Δ A B m s eq tym ihm tyB A1 A2 B0 m0
-      s1 s2 t e eq2 tyB0; subst.
+  { move=>Θ Γ Δ A B m s eq tym ihm tyB A1 A2 B0 m0
+           s1 s2 t e eq2 tyB0; subst.
     apply: ihm...
     apply: conv_trans... }
 Qed.
 
-Lemma dyn_lam1_invX Γ Δ A1 A2 B C m s1 s2 t :
-  Γ ; Δ ⊢ Lam1 A1 m s1 : C ->
+Lemma dyn_lam1_invX Θ Γ Δ A1 A2 B C m s1 s2 t :
+  Θ ; Γ ; Δ ⊢ Lam1 A1 m s1 : C ->
   C === Pi1 A2 B s2 ->
   (A2 :: Γ) ⊢ B : Sort t ->
-  exists r, (A2 :: Γ) ; A2 :{r} Δ ⊢ m : B.
+  exists r, Θ ; (A2 :: Γ) ; A2 :{r} Δ ⊢ m : B.
 Proof with eauto.
   move e:(Lam1 A1 m s1)=>n tyL.
-  elim: tyL A1 A2 B m s1 s2 t e=>//{Γ Δ C n}.
-  { move=>Γ Δ A B m s t k tym _ A1 A2 B0 m0
-      s1 s2 t0[e1 e2 e3]/pi1_inj[eq1[eq2 e4]]tyB0; subst.
+  elim: tyL A1 A2 B m s1 s2 t e=>//{Θ Γ Δ C n}.
+  { move=>Θ Γ Δ A B m s t k1 k2 tym _ A1 A2 B0 m0
+           s1 s2 t0[e1 e2 e3]/pi1_inj[eq1[eq2 e4]]tyB0; subst.
     have wf:=dyn_type_wf tym. inv wf.
     have wf:=sta_type_wf tyB0. inv wf.
     have[A0 rd1 rd2]:=church_rosser eq1.
     have tyA0t:=sta_rd H4 rd1.
     have tyA0s:=sta_rd H3 rd2.
-    have/sort_inj e:=sta_uniq tyA0t tyA0s. subst.
+    have e:=sta_unicity tyA0t tyA0s. subst.
     exists s.
     apply: dyn_ctx_conv1.
     apply: conv_sym...
     exact: H3.
     apply: dyn_conv...
     apply: sta_ctx_conv... }
-  { move=>Γ Δ A B m s eq tym ihm tyB A1 A2 B0 m0
-      s1 s2 t e eq2 tyB0; subst.
+  { move=>Θ Γ Δ A B m s eq tym ihm tyB A1 A2 B0 m0
+           s1 s2 t e eq2 tyB0; subst.
     apply: ihm...
     apply: conv_trans... }
 Qed.
 
-Lemma dyn_lam0_inv Γ Δ m A1 A2 B s1 s2 :
-  Γ ; Δ ⊢ Lam0 A2 m s2 : Pi0 A1 B s1 -> (A1 :: Γ) ; _: Δ ⊢ m : B.
+Lemma dyn_lam0_inv Θ Γ Δ m A1 A2 B s1 s2 :
+  Θ ; Γ ; Δ ⊢ Lam0 A2 m s2 : Pi0 A1 B s1 -> Θ ; (A1 :: Γ) ; _: Δ ⊢ m : B.
 Proof with eauto.
   move=>ty.
   have[t/sta_pi0_inv[r[tyB _]]]:=dyn_valid ty.
   apply: dyn_lam0_invX...
 Qed.
 
-Lemma dyn_lam1_inv Γ Δ m A1 A2 B s1 s2 :
-  Γ ; Δ ⊢ Lam1 A2 m s2 : Pi1 A1 B s1 -> exists r, (A1 :: Γ) ; A1 :{r} Δ ⊢ m : B.
+Lemma dyn_lam1_inv Θ Γ Δ m A1 A2 B s1 s2 :
+  Θ ; Γ ; Δ ⊢ Lam1 A2 m s2 : Pi1 A1 B s1 -> exists r, Θ ; (A1 :: Γ) ; A1 :{r} Δ ⊢ m : B.
 Proof with eauto.
   move=>ty.
   have[t/sta_pi1_inv[r[tyB _]]]:=dyn_valid ty.
   apply: dyn_lam1_invX...
 Qed.
+
+Lemma dyn_pair0_invX Θ Γ Δ A B m n s r t C :
+  Θ ; Γ ; Δ ⊢ Pair0 m n s : C ->
+  C === Sig0 A B r ->
+  Γ ⊢ Sig0 A B r : Sort t ->
+  s = r /\ Γ ⊢ m : A /\ Θ ; Γ ; Δ ⊢ n : B.[m/].
+Proof with eauto.
+  move e:(Pair0 m n s)=>x ty.
+  elim: ty A B m n s r t e=>//{Θ Γ Δ x C}.
+  { move=>Θ Γ Δ A B m n t ty1 tym ihm tyn A0 B0 m0 n0 s r t0[e1 e2 e3]
+      /sig0_inj[e4[e5 e6]]ty2; subst.
+    have[s[r0[ord[tyA0[tyB0/sort_inj e]]]]]:=sta_sig0_inv ty2. subst.
+    have tym0: Γ ⊢ m : A0 by apply: sta_conv; eauto.
+    repeat split...
+    apply: dyn_conv.
+    apply: sta_conv_subst.
+    all: eauto.
+    apply: sta_esubst...
+    by autosubst. }
+  { move=>Θ Γ Δ A B m s eq tym ihm tyB A0 B0 m0 n s0 r t e eq' ty.
+    apply: ihm...
+    apply: conv_trans... }
+Qed.
+
+Lemma dyn_pair1_invX Θ Γ Δ A B m n s r t C :
+  Θ ; Γ ; Δ ⊢ Pair1 m n s : C ->
+  C === Sig1 A B r ->
+  Γ ⊢ Sig1 A B r : Sort t ->
+  exists Θ1 Θ2 Δ1 Δ2,
+    s = r /\
+    Θ1 ∘ Θ2 => Θ /\
+    Δ1 ∘ Δ2 => Δ /\
+    Θ1 ; Γ ; Δ1 ⊢ m : A /\
+    Θ2 ; Γ ; Δ2 ⊢ n : B.[m/].
+Proof with eauto.
+  move e:(Pair1 m n s)=>x ty.
+  elim: ty A B m n s r t e=>//{Θ Γ Δ x C}.
+  { move=>Θ1 Θ2 Θ Γ Δ1 Δ2 Δ A B m n t mrg1 mrg2 ty1 tym _ tyn _ A0 B0 m0 n0 s r t0
+      [e1 e2 e3]/sig1_inj[e4[e5 e6]]ty2; subst.
+    exists Θ1. exists Θ2. exists Δ1. exists Δ2.
+    have[s[r0[ord1[ord2[tyA0[tyB0/sort_inj e]]]]]]:=sta_sig1_inv ty2. subst.
+    have tym0:Θ1; Γ ; Δ1 ⊢ m : A0 by apply: dyn_conv; eauto.
+    repeat split...
+    apply: dyn_conv.
+    apply: sta_conv_subst.
+    all: eauto.
+    apply: sta_esubst...
+    by autosubst. }
+  { move=>Θ Γ Δ A B m s eq tym ihm tyB A0 B0 m0 n s0 r t e eq' ty.
+    apply: ihm...
+    apply: conv_trans... }
+Qed.
+
+Lemma dyn_pair0_inv Θ Γ Δ A B m n s r :
+  Θ ; Γ ; Δ ⊢ Pair0 m n s : Sig0 A B r ->
+  s = r /\ Γ ⊢ m : A /\ Θ ; Γ ; Δ ⊢ n : B.[m/].
+Proof with eauto.
+  move=>ty.
+  have[t tyS]:=dyn_valid ty.
+  apply: dyn_pair0_invX...
+Qed.
+
+Lemma dyn_pair1_inv Θ Γ Δ A B m n s r :
+  Θ ; Γ ; Δ ⊢ Pair1 m n s : Sig1 A B r ->
+  exists Θ1 Θ2 Δ1 Δ2,
+    s = r /\
+    Θ1 ∘ Θ2 => Θ /\ 
+    Δ1 ∘ Δ2 => Δ /\ 
+    Θ1 ; Γ ; Δ1 ⊢ m : A /\
+    Θ2 ; Γ ; Δ2 ⊢ n : B.[m/].
+Proof with eauto.
+  move=>ty.
+  have[t tyS]:=dyn_valid ty.
+  apply: dyn_pair1_invX...
+Qed.
+
+Lemma dyn_return_inv Θ Γ Δ m B :
+  Θ ; Γ ; Δ ⊢ Return m : B ->
+  exists A, Θ ; Γ ; Δ ⊢ m : A /\ B === IO A.
+Proof with eauto.
+  move e:(Return m)=>x ty.
+  elim: ty m e=>//{Θ Γ Δ B x}.
+  { move=>Θ Γ Δ m A tym ihm m0[e]; subst. exists A... }
+  { move=>Θ Γ Δ A B m s eq1 tym ihm tyB m0 e; subst.
+    have[A0[tym0 eq2]]:=ihm _ erefl.
+    exists A0. split...
+    apply: conv_trans.
+    apply: conv_sym...
+    exact: eq2. }
+Qed.
+
+Lemma dyn_app_inv Θ Γ Δ m n C :
+  Θ ; Γ ; Δ ⊢ App m n : C ->
+  exists A B s,
+    (Θ ; Γ ; Δ ⊢ m : Pi0 A B s /\ Γ ⊢ n : A /\ C === B.[n/]) \/
+    (exists Θ1 Θ2 Δ1 Δ2,
+        Θ1 ∘ Θ2 => Θ /\
+        Δ1 ∘ Δ2 => Δ /\
+        Θ1 ; Γ ; Δ1 ⊢ m : Pi1 A B s /\ Θ2 ; Γ ; Δ2 ⊢ n : A /\ C === B.[n/]).
+Proof with eauto.
+  move e:(App m n)=>x ty.
+  elim: ty m n e=>//{Θ Γ Δ x C}.
+  { move=>Θ Γ Δ A B m n s tym ihm tyn m0 n0[e1 e2]; subst.
+    exists A. exists B. exists s. left. split... }
+  { move=>Θ1 Θ2 Θ Γ Δ1 Δ2 Δ A B m n s mrg1 mrg2 tym ihm tyn ihn m0 n0[e1 e2]; subst.
+    exists A. exists B. exists s. right. exists Θ1. exists Θ2. exists Δ1. exists Δ2. split... }
+  { move=>Θ Γ Δ A B m s eq1 tym ihm tyB m0 n0 e; subst.
+    have [A0[B0[s0[[tym0[tyn0 eq2]]
+                  |[Θ1[Θ2[Δ1[Δ2[mrg1[mrg2[tym0[tyn0 eq2]]]]]]]]]]]]:=ihm _ _ erefl.
+    { exists A0. exists B0. exists s0. left. repeat split...
+      apply: conv_trans.
+      apply: conv_sym...
+      exact: eq2. }
+    { exists A0. exists B0. exists s0. right. exists Θ1. exists Θ2. exists Δ1. exists Δ2. repeat split...
+      apply: conv_trans.
+      apply: conv_sym...
+      exact: eq2. } }
+Qed.
+
+Lemma dyn_tt_inv Θ Γ Δ A : Θ ; Γ ; Δ ⊢ TT : A -> dyn_empty Θ.
+Proof with eauto. move e:(TT)=>m ty. elim: ty e=>//{Θ Γ Δ A}. Qed.
+
+Lemma dyn_ff_inv Θ Γ Δ A : Θ ; Γ ; Δ ⊢ FF : A -> dyn_empty Θ.
+Proof with eauto. move e:(FF)=>m ty. elim: ty e=>//{Θ Γ Δ A}. Qed.
+  
