coq_session/dyn_sr.v
@@ -6,8 +6,32 @@ Set Implicit Arguments.
 Unset Strict Implicit.
 Unset Printing Implicit Defensive.
 
-Lemma dyn_sta_step m n : m ~>> n -> m ~> n.
-Proof with eauto using sta_step. elim... Qed.
+Lemma dyn_sta_step m n A :
+  nil ⊢ m : A -> m ~>> n -> m ~>* n.
+Proof with eauto using sta_step, star1 with sta_red_congr.
+  move e:(nil)=>Γ ty. elim: ty e n=>{Γ m A}.
+  all: try solve[intros;
+                 match goal with
+                 | [ H : _ ~>> _ |- _ ] => inv H
+                 end].
+  { move=>Γ A B m n s tym ihm tyn ihn e n0 st. inv st... }
+  { move=>Γ A B m n s tym ihm tyn ihn e n0 st. inv st... }
+  { move=>Γ A B m n t tyS ihS tym ihm tyn ihn e n0 st. inv st... }
+  { move=>Γ A B m n t tyS ihS tym ihm tyn ihn e n0 st. inv st... }
+  { move=>Γ A B C m n s t tyC ihC tym ihm tyn ihn e n0 st. inv st... }
+  { move=>Γ A B C m n s t tyC ihC tym ihm tyn ihn e n0 st. inv st... }
+  { move=>Γ A m tym ihm e n0 st. inv st... }
+  { move=>Γ A m n1 n2 s tyA ihA tym ihm tyn1 ihn1 tyn2 ihn2 e n st. inv st... }
+  { move=>Γ m A tym ihm e n st. inv st... }
+  { move=>Γ m n A B s tyB ihB tym ihm tyn ihn e n0 st. inv st... }
+  { move=>Γ r1 r2 A B m xor tym ihm e n st. inv st... }
+  { move=>Γ r1 r2 A B m xor tym ihm e n st. inv st... }
+  { move=>Γ r1 r2 A B m xor tym ihm e n st. inv st... }
+  { move=>Γ r1 r2 A B m xor tym ihm e n st. inv st... }
+  { move=>Γ r1 r2 m xor tym ihm e n st. inv st... }
+  { move=>Γ r1 r2 m xor tym ihm e n st. inv st... }
+  { move=>Γ A B m s eq tym ihm tyB ihB e n st. subst... }
+Qed.
 
 Lemma dyn_has_type Γ Δ x s A :
   dyn_has Δ x s A -> dyn_wf Γ Δ -> Γ ⊢ A : Sort s.
@@ -34,46 +58,103 @@ Proof with eauto using key, key_impure.
   { move=>Δ A x [|] hs k... }
 Qed.
 
-Lemma dyn_val_key Γ Δ m A s :
-  Γ ; Δ ⊢ m : A -> Γ ⊢ A : Sort s -> dyn_val m -> Δ ▷ s.
-Proof with eauto using key_impure.
+Lemma dyn_val_stability Θ Γ Δ m A s :
+  Θ ; Γ ; Δ ⊢ m : A -> Γ ⊢ A : Sort s -> dyn_val m -> Θ ▷ s /\ Δ ▷ s.
+Proof with eauto using key_impure, key_empty, key_merge.
   destruct s...
-  move=>ty. elim: ty=>{Γ Δ m A}.
-  { move=>Γ Δ x s A shs dhs wf tyA vl.
-    have tyAs:=dyn_has_type wf shs.
-    have/sort_inj e:=sta_uniq tyA tyAs. subst.
-    apply: dyn_has_key... }
-  { move=>Γ Δ A B m s k tym ih tyP vl.
-    have[_[_/sort_inj->//]]:=sta_pi0_inv tyP. }
-  { move=>Γ Δ A B m s t k tym ih tyP vl.
-    have[_[_/sort_inj->//]]:=sta_pi1_inv tyP. }
-  { move=>Γ Δ A B m n s tym ih tyn tyB vl. inv vl. }
-  { move=>Γ Δ1 Δ2 Δ A B m n s mrg tym ihm tyn ihn tyB vl. inv vl. }
-  { move=>Γ Δ A B m s eq tym ihm tyB1 tyB2 vl.
+  move=>ty. elim: ty=>{Θ Γ Δ m A}...
+  { move=>Θ Γ Δ x s A emp wf shs dhs tyA vl.
+    have tyAs:=dyn_has_type dhs wf.
+    have e:=sta_unicity tyA tyAs. subst.
+    split... apply: dyn_has_key... }
+  { move=>Θ Γ Δ A B m s k1 k2 tym ihm tyP vl.
+    have[_[_/sort_inj e]]:=sta_pi0_inv tyP. subst... }
+  { move=>Θ Γ Δ A B m s t k1 k2 tym ihm tyP vl.
+    have[_[_/sort_inj e]]:=sta_pi1_inv tyP. subst... }
+  { move=>Θ Γ Δ A B m n s tym ihm tyn tyB vl. inv vl. }
+  { move=>Θ1 Θ2 Θ Γ Δ1 Δ2 Δ A B m n s mrg1 mrg2 tym ihm tyn ihn tyB vl. inv vl. }
+  { move=>Θ Γ Δ A B m n t tyS1 tym tyn ihn tyS2 vl.
+    have[s[r[ord[tyA[tyB/sort_inj e]]]]]:=sta_sig0_inv tyS2. subst.
+    inv ord. inv vl.
+    apply: ihn...
+    apply: sta_esubst...
+    by autosubst. }
+  { move=>Θ1 Θ2 Θ Γ Δ1 Δ2 Δ A B m n t mrg1 mrg2 tyS1 tym ihm tyn ihn tyS2 vl.
+    have[s[r[ord1[ord2[tyA[tyB/sort_inj e]]]]]]:=sta_sig1_inv tyS2. subst.
+    inv ord1. inv ord2. inv vl.
+    have[k1 k2]:=ihm tyA H1.
+    have[k3 k4]:=ihn (sta_subst tyB (dyn_sta_type tym)) H3.
+    split... }
+  { move=>Θ1 Θ2 Θ Γ Δ1 Δ2 Δ A B C m n s r t mrg1 mrg2 tyC1 tym ihm tyn ihn tyC2 vl. inv vl. }
+  { move=>Θ1 Θ2 Θ Γ Δ1 Δ2 Δ A B C m n s r1 r2 t mrg1 mrg2 tyC1 tym ihm tyn ihn tyC2 vl. inv vl. }
+  { move=>Θ1 Θ2 Θ Γ Δ1 Δ2 Δ A m n1 n2 s mrg1 mrg2 tyA tym ihm tyn1 ihn1 tyn2 ihn2 ty vl. inv vl. }
+  { move=>Θ Γ Δ m A tym ihm ty vl.
+    have[_[_/sort_inj e]]//:=sta_io_inv ty. }
+  { move=>Θ1 Θ2 Θ Γ Δ1 Δ2 Δ m n A B s t mrg1 mrg2 tyB tym ihm tyn ihn ty vl.
+    have[_[_/sort_inj e]]//:=sta_io_inv ty. }
+  { move=>Θ Γ Δ r x A js wf k tyA ty vl.
+    have[_/sort_inj e]//:=sta_ch_inv ty. }
+  { move=>Θ Γ Δ m A tym ihm ty vl.
+    have[_[_/sort_inj e]]//:=sta_io_inv ty. }
+  { move=>Θ Γ Δ r1 r2 A B m xor tym ihm ty vl.
+    have[_[_/sort_inj e]]//:=sta_io_inv ty. }
+  { move=>Θ Γ Δ r1 r2 A B m xor tym ihm ty vl.
+    have[_[_/sort_inj e]]//:=sta_io_inv ty. }
+  { move=>Θ Γ Δ r1 r2 A B m xor tym ihm ty vl.
+    have[_[_/sort_inj e]]//:=sta_pi0_inv ty. }
+  { move=>Θ Γ Δ r1 r2 A B m xor tym ihm ty vl.
+    have[_[_/sort_inj e]]//:=sta_pi1_inv ty. }
+  { move=>Θ Γ Δ r1 r2 m xor tym ihm ty vl.
+    have[_[_/sort_inj e]]//:=sta_io_inv ty. }
+  { move=>Θ Γ Δ r1 r2 m xor tym ihm ty vl.
+    have[_[_/sort_inj e]]//:=sta_io_inv ty. }
+  { move=>Θ Γ Δ A B m s eq tym ihm tyB1 tyB2 vl.
     have[r tyA]:=dyn_valid tym.
     have[C rd1 rd2]:=church_rosser eq.
     apply: ihm...
     have tyCr:=sta_rd tyA rd1.
     have tyCU:=sta_rd tyB2 rd2.
-    have/sort_inj<-:=sta_uniq tyCr tyCU... }
+    have<-:=sta_unicity tyCr tyCU... }
 Qed.
 
-Theorem dyn_sr Γ Δ m n A :
-  Γ ; Δ ⊢ m : A -> m ~>> n -> Γ ; Δ ⊢ n : A.
-Proof with eauto using dyn_type, dyn_step, dyn_wf.
-  move=>ty. elim: ty n=>{Γ Δ m A}...
-  { move=>Γ Δ x s A wf shs dhs n st. inv st. }
-  { move=>Γ Δ A B m s k tym ihm n st. inv st. }
-  { move=>Γ Δ A B m s t k tym ihm n st. inv st. }
-  { move=>Γ Δ A B m n s tym ihm tyn n0 st. inv st.
-    { have tym':=ihm _ H2.
+Lemma dyn_pure_empty Θ Γ Δ m A :
+  Θ ; Γ ; Δ ⊢ m : A -> Θ ▷ U -> dyn_empty Θ.
+Proof with eauto using dyn_empty, merge_empty.
+  elim=>{Θ Γ Δ m A}...
+  { move=>Θ1 Θ2 Θ Γ Δ1 Δ2 Δ A B m n s mrg1 mrg2 tym ihm tyn ihn k.
+    have[k1 k2]:=pure_split mrg1 k... }
+  { move=>Θ1 Θ2 Θ Γ Δ1 Δ2 Δ A B m n s mrg1 mrg2 tyS tym ihm tyn ihn k.
+    have[k1 k2]:=pure_split mrg1 k... }
+  { move=>Θ1 Θ2 Θ Γ Δ1 Δ2 Δ A B C m n s r t mrg1 mrg2 tyC tym ihm tyn ihn k.
+    have[k1 k2]:=pure_split mrg1 k... }
+  { move=>Θ1 Θ2 Θ Γ Δ1 Δ2 Δ A B C m n s r1 r2 t mrg1 mrg2 tyC tym ihm tyn ihn k.
+    have[k1 k2]:=pure_split mrg1 k... }
+  { move=>Θ1 Θ2 Θ Γ Δ1 Δ2 Δ A m n1 n2 s mrg1 mrg2 tyA tym ihm tyn1 ihn1 tyn2 ihn2 k.
+    have[k1 k2]:=pure_split mrg1 k... }
+  { move=>Θ1 Θ2 Θ Γ Δ1 Δ2 Δ m n A B s t mrg1 mrg2 tyB tym ihm tyn ihn k.
+    have[k1 k2]:=pure_split mrg1 k... }
+  { move=>Θ Γ Δ r x A js wf k1 tyA k2.
+    exfalso. apply: pure_just... }
+Qed.
+
+Theorem dyn_sr Θ m n A :
+  Θ ; nil ; nil ⊢ m : A -> m ~>> n -> Θ ; nil ; nil ⊢ n : A.
+Proof with eauto using dyn_type, dyn_step, dyn_wf, merge.
+  move e1:(nil)=>Γ.
+  move e2:(nil)=>Δ ty. elim: ty e1 e2 n=>{Θ Γ Δ m A}...
+  { move=>Θ Γ Δ x s A emp wf shs dhs e1 e2 n st. inv st. }
+  { move=>Θ Γ Δ A B m s k1 k2 tym ihm e1 e2 n st. inv st. }
+  { move=>Θ Γ Δ A B m s t k1 k2 tym ihm e1 e2 n st. inv st. }
+  { move=>Θ Γ Δ A B m n s tym ihm tyn e1 e2 n0 st. inv st.
+    { have tym':=ihm erefl erefl _ H2.
       apply: dyn_app0... }
-    { have tyn':=sta_sr tyn (dyn_sta_step H2).
+    { have tyn':=sta_rd tyn (dyn_sta_step tyn H2).
       have[t tyP]:=dyn_valid tym.
       have[r[tyB _]]:=sta_pi0_inv tyP.
       apply: dyn_conv.
       apply: sta_conv_beta.
-      apply: conv1i.
+      apply: conv_sym.
+      apply: star_conv.
       apply: dyn_sta_step...
       apply: dyn_app0...
       have:=sta_subst tyB tyn.
@@ -82,36 +163,131 @@ Proof with eauto using dyn_type, dyn_step, dyn_wf.
       have tym0:=dyn_lam0_inv tym.
       apply: dyn_subst0... }
     { exfalso.
-      apply: sta_lam1_pi0_false...
-      apply: dyn_sta_type... } }
-  { move=>Γ Δ1 Δ2 Δ A B m n s mrg tym ihm tyn ihn n0 st. inv st.
-    { have tym':=ihm _ H2.
+      apply: sta_lam1_pi0_false... } }
+  { move=>Θ1 Θ2 Θ Γ Δ1 Δ2 Δ A B m n s mrg1 mrg2 tym ihm tyn ihn e1 e2 n0 st.
+    subst. inv mrg2. inv st.
+    { have tym':=ihm erefl erefl _ H2.
       apply: dyn_app1... }
-    { have tyn':=ihn _ H2.
+    { have tyn':=ihn erefl erefl _ H2.
       have[x tyP]:=dyn_valid tym.
       have[r[tyB _]]:=sta_pi1_inv tyP.
       apply: dyn_conv.
       apply: sta_conv_beta.
-      apply: conv1i.
+      apply: conv_sym.
+      apply: star_conv.
       apply: dyn_sta_step...
       apply: dyn_app1...
       have:=sta_subst tyB (dyn_sta_type tyn).
       asimpl... }
     { exfalso.
-      apply: sta_lam0_pi1_false...
-      apply: dyn_sta_type... }
+      apply: sta_lam0_pi1_false... }
     { have[x tyP]:=dyn_valid tym.
       have[r[tyB _]]:=sta_pi1_inv tyP.
       have[t tym0]:=dyn_lam1_inv tym.
       have wf:=dyn_type_wf tym0. inv wf.
-      apply: dyn_subst1...
-      apply: dyn_val_key... } }
+      have[k1 k2]:=dyn_val_stability tyn H5 H2.
+      apply: dyn_subst1.
+      apply: k1. apply: mrg1. apply: k2. apply: merge_nil.
+      all: eauto. } }
+  { move=>Θ Γ Δ A B m n t tyS tym ihm tyn e1 e2 n0 st. inv st.
+    have[s[r[ord[tyA[tyB _]]]]]:=sta_sig0_inv tyS.
+    apply: dyn_pair0... }
+  { move=>Θ1 Θ2 Θ Γ Δ1 Δ2 Δ A B m n t mrg1 mrg2 tyS tym ihm tyn ihn e1 e2 n0 st.
+    subst. inv mrg2. inv st.
+    { have[s[r[ord1[ord2[tyA[tyB _]]]]]]:=sta_sig1_inv tyS.
+      apply: dyn_pair1...
+      apply: dyn_conv.
+      apply: sta_conv_beta.
+      apply: star_conv.
+      apply: (dyn_sta_step (dyn_sta_type tym))...
+      apply: tyn.
+      apply: sta_esubst...
+      by autosubst. }
+    { apply: dyn_pair1... } }
+  { move=>Θ1 Θ2 Θ Γ Δ1 Δ2 Δ A B C m n s r t mrg1 mrg2 tyC tym ihm tyn ihn e1 e2 n0 st.
+    subst. inv mrg2. inv st.
+    { apply: dyn_conv.
+      apply: sta_conv_beta.
+      apply: conv_sym.
+      apply: star_conv.
+      apply: (dyn_sta_step (dyn_sta_type tym))...
+      apply: dyn_letin0...
+      apply: sta_esubst...
+      by autosubst. }
+    { inv H3.
+      have[e[tym1 tym2]]:=dyn_pair0_inv tym. subst.
+      have wf:=dyn_type_wf tyn. inv wf. inv H3.
+      have[k1 k2]:=dyn_val_stability tym2 (sta_subst H5 tym1) H0.
+      have[Θ0[emp mrg0]]:=dyn_type_empty tym2.
+      replace C.[Pair0 m1 m2 t/]
+        with C.[Pair0 (Var 1) (Var 0) t .: ren (+2)].[m2,m1/] by autosubst.
+      apply: dyn_substitution...
+      apply: (dyn_agree_subst_wk1 k1 k2)...
+      apply: dyn_agree_subst_wk0...
+      by autosubst. }
+    { exfalso. apply: sta_pair1_sig0_false... } }
+  { move=>Θ1 Θ2 Θ Γ Δ1 Δ2 Δ A B C m n s r1 r2 t mrg1 mrg2 tyC tym ihm tyn ihn e1 e2 n0 st.
+    subst. inv mrg2. inv st.
+    { apply: dyn_conv.
+      apply: sta_conv_beta.
+      apply: conv_sym.
+      apply: star_conv.
+      apply: (dyn_sta_step (dyn_sta_type tym))...
+      apply: dyn_letin1...
+      apply: sta_esubst...
+      by autosubst. }
+    { exfalso. apply: sta_pair0_sig1_false... }
+    { inv H3.
+      have[Θ1'[Θ2'[Δ1'[Δ2'[e[mrg1'[mrg2'[tym1 tym2]]]]]]]]:=dyn_pair1_inv tym.
+      have wf:=dyn_type_wf tyn. inv wf. inv H3. inv mrg2'.
+      have[Θ0[emp mrg0]]:=dyn_type_empty tym1.
+      have [k1 k2]:=dyn_val_stability tym1 H8 H1.
+      have [k3 k4]:=dyn_val_stability tym2 (sta_subst H6 (dyn_sta_type tym1)) H4.
+      replace C.[Pair1 m1 m2 t/]
+        with C.[Pair1 (Var 1) (Var 0) t .: ren (+2)].[m2,m1/] by autosubst.
+      apply: dyn_substitution...
+      apply: (dyn_agree_subst_wk1 k3 k4)...
+      apply: (dyn_agree_subst_wk1 k1 k2)...
+      by autosubst. } }
+  { move=>Θ Γ Δ A m k1 k2 tym ihm e1 e2 n st. subst. inv st.
+    have tyF:=dyn_fix k1 k2 tym.
+    have mrg:=pure_merge_self k1.
+    have:=dyn_subst1 k1 mrg k2 merge_nil tym tyF.
+    by autosubst. }
+  { move=>Θ Γ Δ emp wf k e1 e2 n st. inv st. }
+  { move=>Θ Γ Δ emp wf k e1 e2 n st. inv st. }
+  { move=>Θ Γ Δ emp wf k e1 e2 n st. inv st. }
+  { move=>Θ1 Θ2 Θ Γ Δ1 Δ2 Δ A m n1 n2 s mrg1 mrg2 tyA tym ihm tyn1 ihn1 tyn2 ihn2 e1 e2 n st.
+    subst. inv mrg2. inv st.
+    { have tym':=ihm erefl erefl _ H4.
+      apply: dyn_conv.
+      apply: sta_conv_beta.
+      apply: conv_sym.
+      apply: star_conv.
+      apply: dyn_sta_step...
+      apply: dyn_ifte...
+      apply: sta_subst tyA (dyn_sta_type tym). }
+    { have emp:=dyn_tt_inv tym.
+      have e:=merge_emptyL mrg1 emp. subst... }
+    { have emp:=dyn_ff_inv tym.
+      have e:=merge_emptyL mrg1 emp. subst... } }
+  { move=>Θ Γ Δ m A tym ihm e1 e2 n st. inv st... }
+  { move=>Θ1 Θ2 Θ Γ Δ1 Δ2 Δ m n A B s t mrg1 mrg2 tyB tym ihm tyn ihn e1 e2 n0 st.
+    subst. inv mrg2. inv st... }
+  { move=>Θ Γ Δ r x A js wf k tyA e1 e2 n st. inv st. }
+  { move=>Θ Γ Δ m A tym ihm e1 e2 n st. inv st. }
+  { move=>Θ Γ Δ r1 r2 A B m xor tym ihm e1 e2 n st. inv st... }
+  { move=>Θ Γ Δ r1 r2 A B m xor tym ihm e1 e2 n st. inv st... }
+  { move=>Θ Γ Δ r1 r2 A B m xor tym ihm e1 e2 n st. inv st... }
+  { move=>Θ Γ Δ r1 r2 A B m xor tym ihm e1 e2 n st. inv st... }
+  { move=>Θ Γ Δ r1 r2 m xor tym ihm e1 e2 n st. inv st... }
+  { move=>Θ Γ Δ r1 r2 m xor tym ihm e1 e2 n st. inv st... }
 Qed.
 
-Corollary dyn_rd Γ Δ m n A :
-  Γ ; Δ ⊢ m : A -> m ~>>* n -> Γ ; Δ ⊢ n : A.
+Corollary dyn_rd Θ m n A :
+  Θ ; nil ; nil ⊢ m : A -> m ~>>* n -> Θ ; nil ; nil ⊢ n : A.
 Proof with eauto.
-  move=>ty rd. elim: rd Γ A ty=>{n}...
+  move=>ty rd. elim: rd Θ A ty=>{n}...
   move=>n z rd ih st Γ A tym.
   have tyn:=ih _ _ tym.
   apply: dyn_sr...
